One more field in the `regional` typeclass (`r_init_p`)

secure_api/merkle_tree/Low.RVector.Instances.fst
@@ -1,9 +1,9 @@
-module LowStar.RVector.Instances
+module Low.RVector.Instances
 
 open FStar.All
 open FStar.Integers
 open LowStar.Buffer
-open LowStar.RVector
+open Low.RVector
 
 module HH = FStar.Monotonic.HyperHeap
 module HS = FStar.HyperStack
@@ -11,8 +11,8 @@ module HST = FStar.HyperStack.ST
 module MHS = FStar.Monotonic.HyperStack
 module S = FStar.Seq
 module B = LowStar.Buffer
-module V = LowStar.Vector
-module RV = LowStar.RVector
+module V = Low.Vector
+module RV = Low.RVector
 
 /// `LowStar.Buffer` is regional
 
@@ -66,6 +66,11 @@ val buffer_irepr:
 let buffer_irepr #a ia len =
   Ghost.hide (S.create (UInt32.v len) ia)
 
+val buffer_r_init_p:
+  #a:Type0 -> v:B.buffer a -> GTot Type0
+let buffer_r_init_p #a v =
+  True
+
 val buffer_r_init:
   #a:Type -> ia:a -> len:UInt32.t{len > 0ul} -> r:erid ->
   HST.ST (b:B.buffer a)
@@ -74,6 +79,7 @@ val buffer_r_init:
       Set.subset (Map.domain (MHS.get_hmap h0))
                  (Map.domain (MHS.get_hmap h1)) /\
       modifies loc_none h0 h1 /\
+      buffer_r_init_p v /\
       buffer_r_inv len h1 v /\
       buffer_region_of v = r /\
       buffer_r_repr h1 v == Ghost.reveal (buffer_irepr ia len)))
@@ -116,6 +122,7 @@ let buffer_regional #a ia len =
       (buffer_r_inv_reg #a len)
       (buffer_r_sep #a len)
       (buffer_irepr #a ia len)
+      (buffer_r_init_p #a)
       (buffer_r_init #a ia len)
       (buffer_r_free #a len)
 
@@ -174,6 +181,11 @@ val vector_irepr:
 let vector_irepr #a rg =
   Ghost.hide S.empty
 
+val vector_r_init_p:
+  #a:Type -> #rg:regional a -> v:rvector rg -> GTot Type0
+let vector_r_init_p #a #rg v =
+  V.size_of v = 0ul
+
 val vector_r_init: 
   #a:Type -> #rg:regional a -> r:erid ->
   HST.ST (v:rvector rg)
@@ -182,6 +194,7 @@ val vector_r_init:
       Set.subset (Map.domain (MHS.get_hmap h0))
                  (Map.domain (MHS.get_hmap h1)) /\
       modifies loc_none h0 h1 /\
+      vector_r_init_p v /\
       vector_r_inv h1 v /\
       vector_region_of v = r /\
       vector_r_repr h1 v == Ghost.reveal (vector_irepr rg)))
@@ -211,14 +224,7 @@ let vector_regional #a rg =
       (vector_r_inv_reg #a #rg)
       (vector_r_sep #a #rg)
       (vector_irepr #a rg)
+      (vector_r_init_p #a #rg)
       (vector_r_init #a #rg)
       (vector_r_free #a #rg)
-
-// An instantiation: `LowStar.Buffer` of `LowStar.RVector` is regional.
-
-val buffer_vector_regional:
-  #a:Type -> ia:a -> len:UInt32.t{len > 0ul} ->
-  regional (rvector #(B.buffer a) (buffer_regional ia len))
-let buffer_vector_regional #a ia len =
-  vector_regional (buffer_regional ia len)
 
